VCVio/OracleComp/ProbComp.lean
@@ -94,7 +94,7 @@ protected def inductionOn {α} {C : ProbComp α → Prop}
     (pure : (a : α) → C (pure a))
     (query_bind : (n : ℕ) → (mx : Fin (n + 1) → ProbComp α) → (∀ m, C (mx m)) → C ($[0..n] >>= mx))
     (oa : ProbComp α) : C oa :=
-  PFunctor.FreeM.inductionOn pure query_bind oa
+  PFunctor.FreeM.induction pure query_bind oa
 
 end uniformFin
 
